Setlec/Verify/Fueled.lean
@@ -230,6 +230,12 @@ theorem reduceNat_atF (d : Nat) (e : Expr) (F : Nat) :
   unfold reduceNat
   atF_tac
 
+theorem boolTrueShortcut_atF (d : Nat) (e : Expr) (F : Nat) :
+    (boolTrueShortcut (fueledFns mode env) d e).val F =
+      boolTrueShortcut (pureFns mode env F) d e := by
+  unfold boolTrueShortcut
+  atF_tac
+
 theorem ensureSort_atF (d : Nat) (e : Expr) (F : Nat) :
     (ensureSort (fueledFns mode env) env d e).val F =
       ensureSort (pureFns mode env F) env d e := by
@@ -307,6 +313,7 @@ macro "atF_step2" : tactic =>
     | (rw [defEqList_atF])
     | (rw [structEtaProjCerts_atF])
     | (rw [reduceNat_atF])
+    | (rw [boolTrueShortcut_atF])
     | (rw [ensureSort_atF])
     | (rw [proofIrrel_atF])
     | (rw [propIrrel_atF])
@@ -397,6 +404,7 @@ macro "atF_step3" : tactic =>
     | (rw [defEqList_atF])
     | (rw [structEtaProjCerts_atF])
     | (rw [reduceNat_atF])
+    | (rw [boolTrueShortcut_atF])
     | (rw [ensureSort_atF])
     | (rw [proofIrrel_atF])
     | (rw [propIrrel_atF])
@@ -443,6 +451,7 @@ macro "atF_core4" x:tactic : tactic =>
     | (rw [defEqList_atF])
     | (rw [structEtaProjCerts_atF])
     | (rw [reduceNat_atF])
+    | (rw [boolTrueShortcut_atF])
     | (rw [ensureSort_atF])
     | (rw [proofIrrel_atF])
     | (rw [propIrrel_atF])
